\documentclass{memoir}
\usepackage{linalg}
\usepackage{marginnote}
\begin{document}
% \section{}	
\section{First Consequences of Axioms of a Vector Space}
Let $(V,F,+,\cdot)$ be a vector space. 
\begin{prop}
The additive identity of $V$ is unique
\end{prop}
\begin{proof}
	Suppose $V$ has two additive identities $\overline{0}, \overline{0'}$. Then $\overline{0} = \overline{0}+ \overline{0'} = \overline{0'}$.
\end{proof}

\begin{prop}
	Additive inverses are unique
\end{prop}

\begin{proof}
	Let $v\in V$ be any vector. Suppose that $w, w'$ are additive inverses of v.
	Then 
	\begin{align*}
		w &= w + \overline{0}\\
		  &= w + (v+w')\\
		  &= (w+v) + w'\\
		  &= \overline{0} + w'\\
		  &= w'
	\end{align*}
\end{proof}

\begin{prop}
	For all $v\in V, 0\cdot v = \overline{0}$
\end{prop}

\begin{proof}
	\begin{align*}
		0 \cdot v &= (0+0) \cdot v\\
			  &= 0\cdot v + 0\cdot v
	\end{align*}
	Add $-0\cdot v$ to both sides:
\begin{align*}
	-(0\cdot v) + (0\cdot v) &= -(0\cdot v) + (0\cdot v) + (0\cdot v)\\
				 &\implies \overline{0} = \overline{0} + (0\cdot v)\\
				 &\implies \overline{0} = 0\cdot v
\end{align*}
\end{proof}

\begin{hw}
	Prove that $-v = (-1)*v$.
\end{hw}
\end{document}
